More text.

Thesis.thy
@@ -21,11 +21,11 @@ On the other hand, there is still an ongoing debate about the most suitable logi
 to be used for the foundations of mathematics (TODO: cite). While higher-order functional type
 theory is closely tied to set theory (see \cite{HigherOrderLogicSetTheoryFalseDilemma}, TODO: rethink citation)
 and set theory has long been a prime choice for a common denominator of mathematical disciplines
-(TODO: cite), it's modern paradox free axiomatization following Zermelo-Fraenkel is often viewed as complex and counter-intuitive,
-respectively lacking in philosophical grounding and justification.
+(TODO: cite), it's modern paradox free axiomatization following Zermelo-Fraenkel is often viewed as
+complex and counter-intuitive, respectively lacking in philosophical grounding and justification (TODO: cite).
 
 While there is prominent research into alternative foundational approaches (e.g. homotopy type
-theory; TODO: cite - maybe something else, since homotopy type theory maps just perfectly to HOL...),
+theory; TODO: cite - maybe something else, since homotopy type theory maps rather nicely to HOL...),
 a potential practical problem for such approaches and a pragmatic defense of set theory as foundation
 is the effort required in building up automated reasoning systems that are on par with the existing
 tools that are available for processing theories grounded in set theory.
@@ -40,8 +40,8 @@ is a particularly interesting target. On the one hand it aims to be a foundation
 that can serve as the basis for mathematics, linguistics and the sciences (TODO: rethink, cite), while
 on the other hand it is based on logical foundations that differ from classical functional higher-order
 theory and were even argued to be incompatible (see \cite{rtt}).
-In our previous work (see \cite{MScThesis}) we demonstrated how our method for formally analysing
-models and semantics for such a system can be beneficial and vital for its soundness.
+In our previous work (see \cite{MScThesis}) we demonstrated how our method for formally analyzing
+models and semantics for such a system can be beneficial and vital for its soundness (TODO: refer to section with details).
 During our continued work we could contribute to the evolution of Abstract Object Theory and
 simultaneously arrived at a faithful representation of its model structure, semantics and
 deductive system in Isabelle/HOL that can utilize the existing automated reasoning infrastructure.
@@ -66,7 +66,7 @@ of Anselm's ontological argument (in \cite{OppenheimerZalta2011}, Oppenheimer an
 only one of the three premises they used in \cite{OppenheimerZalta1991} is sufficient) or the
 reconstruction of theorems in Spinoza's \emph{Ethics} in \cite{SpinozaProver9}.
 
-However, there are inherent limitations to the approach of analyzing a higher-order theory like AOT
+However, there are inherent limitations to the approach of analyzing higher-order theories like AOT
 with the help of first-order provers. While it is possible to reason about the first order truth
 conditions of statements by introducing sort predicates and using a number of special techniques
 to translate the statements into the less-expressive language of multi-sorted first-order logic
@@ -86,45 +86,46 @@ to the meta-logic. This is done by reusing as much of the infrastructure of the 
 while \emph{defining} the syntactic elements of the target logic that are not part of
 the meta-logic by means of a representation of their semantics. Since sets have a natural
 representation in higher-order logic, this approach works well for any logical system that
-has a semantics defined in terms of sets.
+has a semantics defined in terms of sets. The approach of shallow semantic embeddings is discussed in
+more detail in chapter~\ref{SSEs}.
 
-In \cite{ModalLogics} Benzm\"uller and Paulson represented quantified modal logic using SSEs by means
-of embedding modal operators based using their Kripke semantics (TODO cite). This allowed for an
+(TODO: citation is embedding in simple type theory, not Isabelle/HOL. Rethink.) In \cite{ModalLogics} Benzm\"uller and Paulson represented quantified modal logic using SSEs by means
+of embedding modal operators based on their Kripke semantics (TODO cite). This allowed for an
 extensive analysis of G\"odel's ontological argument in second-order S5 modal logic (TODO cite), followed
 by a range of studies of similar ontological arguments (TODO cite). TODO: newer work by Benzm\"uller.
 
 The advantage of these studies using SSEs compared to the earlier use of Prover9 is that arguments
-can be represented their native syntax and are thereby readable and maintainable, while the theorem
+can be represented in their native syntax and are thereby readable and maintainable, while the theorem
 proving environments are capable of automatically transforming statements into a suitable first-order
-representation on the fly to allow first-order theorem provers like E or SPASS (TODO: cite) perform
+representation on the fly to allow first-order theorem provers like E or SPASS (TODO: cite) to perform
 proof search much like Prover9 was able to do on a manually constructed first-order representation.
 
 These studies were still mainly concerned with case studies of concrete arguments or
-with only conservative extensions of higher-order logic like functional higher-order modal logic.
+with conservative extensions of higher-order logic like functional higher-order modal logic.
 Furthermore, they relied heavily on the previously available completeness results of second-order modal
-logic with respect to Kripke models.
+logic with respect to Kripke models (TODO: cite).
 
 In our own previous work (in \cite{MScThesis}) we applied an extended version of this technique
-to AOT. For AOT no extensive prior analysis for canonical models - like Kripke models for higher-order
+to AOT. For AOT no extensive prior analysis of canonical models - like Kripke models for higher-order
 modal logic - was available. While the so-called Aczel models of object theory (TODO: cite) provided
 an important building block for constructing models of AOT in HOL, no full set-theoretic model
 of object theory had been constructed. In \cite{MScThesis} we extended the existing Aczel models to
 a richer model structure that was capable of approximating the validity of statements of the most
-recent formulation of AOT. Furthernmore, we introduced the new concept of \emph{abstraction layers}.
-An abstraction layer consists of a derivation of the axioms and deduction rules of a target system
-from a given semantics that is then considered as ground truth while "forgetting" the underlying
-semantic structure (i.e. the reasoning system is prevented from using the semantics for proofs, but
-configured to solely rely on the derived axioms and deduction rules). Abstraction layers turned out
-to be a helpful means for reasoning within a target theory without the danger of deriving artifactual
-theories, even in the absence of a formal completeness result about the used semantics. Furthermore,
-it can be used to analyze soundness and completeness of the semantics itself.
+recent formulation of AOT in Principia Logico-Metaphysica (PLM). Furthermore, we introduced the new
+concept of \emph{abstraction layers}. An abstraction layer consists of a derivation of the axioms and
+deduction rules of a target system from a given semantics that is then considered as ground truth while
+"forgetting" the underlying semantic structure (i.e. the reasoning system is prevented from using the
+semantics for proofs, but configured to solely rely on the derived axioms and deduction rules).
+Abstraction layers turned out to be a helpful means for reasoning within a target theory without
+the danger of deriving artifactual theories, even in the absence of a formal completeness result
+about the used semantics. Furthermore, it can be used to analyze soundness and completeness of the semantics itself.
 
-The final result of \cite{MScThesis} was the discovery of an oversight in the formulation of AOT that
+A major result of \cite{MScThesis} was the discovery of an oversight in the formulation of AOT that
 allowed for the reintroduction of a previously known paradox into the system. While multiple quick
 fixes to restore the consistency of AOT were immediately available, in the aftermath of this result
-AOT was significantly reworked and improved, the aftermath of this result was an extensive debate
-of the foundations of AOT which culminated in the extension of the free logic AOT that was previously
-restricted to its individual terms to account for non-denoting definite descriptions to its relation
+AOT was significantly reworked and improved. The result triggered an extensive debate
+of the foundations of AOT which culminated in the extension of the free logic AOT previously merely
+used for its individual terms to account for non-denoting definite descriptions to its relation
 terms as well. This reworking of AOT was accompanied by a continuous further development of its
 embedding in Isabelle/HOL. This mutually beneficial mode of work was already partly described in
 (TODO cite Open Philosophy) and resulted in a now stabilized improved formulation of AOT and a
@@ -135,8 +136,8 @@ matching embedding. The details of this process and its results is the main subj
 section\<open>Overview of the Following Chapters\<close>
 
 text\<open>
-In the following,  we first give a brief introduction to Abstract Object Theory and
-a more detailed description of Shallow Semantical Embeddings. Based on that we describe the constructed
+In the following,  we first give a more detailed description of Shallow Semantical Embeddings and
+a brief introduction to Abstract Object Theory. Based on that we describe the constructed
 embedding of Abstract Object Theory in Isabelle/HOL while highlighting the contributions
 of the embedding to the theory of abstract objects on the one hand and the techniques developed for
 its implementation on the other hand. Finally we present the results on Natural Numbers and
@@ -145,14 +146,112 @@ type-theoretic version of Abstract Object Theory.
 \<close>
 
 
-chapter\<open>Shallow Semantic Embeddings\<close>
+chapter\<open>Shallow Semantic Embeddings\<close>text\<open>\label{SSEs}\<close>
 
-section\<open>History\<close>
+section\<open>Embeddings of Domain-Specific Languages\<close>
 text\<open>
+
+In computer science, deep and shallow embeddings have been a traditional means to implement domain-specific
+languages by embedding them into general-purpose host languages (see for example \cite{DomainSpecificLanguages}).
+A simple example is a language of \emph{expressions} that can be either integer constants, resp. literals
+or the addition of two other expressions.
+If we consider Isabelle/HOL as the host language in this process, the following would constitute a
+\emph{deep} embedding of this language:
+\<close>
+
+(*<*)
+locale Deep
+begin
+(*>*)
+
+datatype expression = Literal int | Addition expression expression
+primrec eval :: \<open>expression \<Rightarrow> int\<close> where
+        \<open>eval (Literal x) = x\<close>
+      | \<open>eval (Addition x y) = eval x + eval y\<close>
+
+(*<*)
+lemma CommutativeAdditionNonIdentity: \<open>Addition x y \<noteq> Addition y x\<close> if \<open>x \<noteq> y\<close>
+  using that Deep.expression.inject(2) by auto
+lemma CommutativeAdditionEquivalent: \<open>eval (Addition x y) = eval (Addition y x)\<close>
+  by simp
+end
+(*>*)
+
+text\<open>
+The deep embedding consists of a (usually recursive) algebraic datatype that captures the syntax of
+the language to be embedded. This syntax is then given a semantics by means of an evaluation function
+that traverses this algebraic datatype.
+A shallow embedding on the other hand, represents the syntactic elements of a target language directly
+by its semantics. In our example, the semantic domain of expressions is the integers. Then the
+operations on the expressions are \emph{defined} directly by means of their semantics:
+\<close>
+
+(*<*)
+locale Shallow
+begin
+(*>*)
+
+type_synonym expression = int
+definition Literal :: \<open>int \<Rightarrow> expression\<close> where \<open>Literal x \<equiv> x\<close>
+definition Addition :: \<open>expression \<Rightarrow> expression \<Rightarrow> expression\<close> where \<open>Addition x y \<equiv> x + y\<close>
+
+(*<*)
+lemma CommutativeAdditionIdentity: \<open>Addition x y = Addition y x\<close>
+  by (simp add: Shallow.Addition_def)
+end
+
+lemma Deep_Shallow_Literal: \<open>Deep.eval (Deep.Literal x) = Shallow.Literal x\<close>
+  by (simp add: Deep.eval.simps(1) Shallow.Literal_def)
+
+lemma Deep_Shallow_Addition: \<open>Deep.eval (Deep.Addition x y) = Shallow.Addition (Deep.eval x) (Deep.eval y)\<close>
+  by (simp add: Deep.eval.simps(2) Shallow.Addition_def)
+
+(*>*)
+
+text\<open>
+Note that in the shallow embedding, the domain of \emph{expression}s is in fact shared with the
+meta-language by directly representing expressions in the type to which they evaluate semantically
+in the deep embedding, namely \emph{int} in the example.
+
+There is a natural correspondence between the deep and shallow representations of this
+language. In particular @{thm[show_question_marks = false, names_short = false] Deep_Shallow_Literal} and
+@{thm[show_question_marks = false, names_short = false] Deep_Shallow_Addition} hold. So the semantic
+evaluation is implicit in the shallow embedding.
+On the other hand there are also differences between the two representation. For example, in the
+deep embedding adding \emph{x} to \emph{y} results in an expression that is different from adding
+\emph{y} to \emph{x} for distinct \emph{x} and \emph{y}, even though they are equivalent under evaluation:
+
+@{thm[show_question_marks = false, names_short = false, display = true] Deep.CommutativeAdditionNonIdentity}
+@{thm[show_question_marks = false, names_short = false, display = true] Deep.CommutativeAdditionEquivalent}
+
+In contrast, the two additions are actually identical in the shallow embedding:
+
+@{thm[show_question_marks = false, names_short = false, display = true] Shallow.CommutativeAdditionIdentity}
+
+In fact, the shallow embedding can be thought of as a \emph{quotient} of the deep embedding under
+semantic evaluation. TODO: something formal about this?
+
+While there are several advantages and disadvantages of using shallow vs. deep embeddings for
+Domain-Specific languages, we forgo a detailed discussion of them here (TODO: maybe citation?) and
+focus on the application of similar modes of embeddings to logical reasoning in the next section.
+\<close>
+
+section\<open>SSEs as Universal Reasoning Tools\<close>
+
+text\<open>
+
+In \cite{UniversalReasoning}, Benzm\"uller develops the idea of using \emph{Shallow Semantic Embeddings} (SSEs)
+in classical higher-order logics as a means for universal reasoning. TODO: paraphraze the idea a bit.
+
 \<close>
 
 section\<open>SSE of Quantified Higher-Order Modal Logic\<close>
 text\<open>
+
+An example for non-classical logics that are used prominently in metaphysics is Quantified Higher-Order
+Modal Logic. In \cite{ModalLogics} Benzm\"uller and Paulson develop a sound and complete embedding
+of quantified higher-order modal logic into simple type theory.
+
 \<close>
 
 chapter\<open>Abstract Object Theory\<close>
@@ -160,6 +259,9 @@ chapter\<open>Abstract Object Theory\<close>
 section\<open>Overview and Motivation\<close>
 
 text\<open>
+
+Abstract Object Theory (AOT or \emph{object theory}) is a meta-physical theory inspired by ideas of
+Ernst Mally and formalized by Edward Zalta. 
 
 \<close>
 
